src/Separation_Rename.thy
@@ -6,7 +6,7 @@ begin
 
 lemmas apply_fun = apply_iff[THEN iffD1]
 
-lemma nth_concat : "[p,t] \<in> list(A) \<Longrightarrow> env\<in> list(A) \<Longrightarrow> nth(1 #+ length(env),[p]@ env @ [t]) = t"
+lemma nth_concat : "[p,t] \<in> list(A) \<Longrightarrow> env\<in> list(A) \<Longrightarrow> nth(1 +\<^sub>\<omega> length(env),[p]@ env @ [t]) = t"
   by(auto simp add:nth_append)
 
 lemma nth_concat2 : "env\<in> list(A) \<Longrightarrow> nth(length(env),env @ [p,t]) = p"
@@ -17,76 +17,76 @@ lemma nth_concat3 : "env\<in> list(A) \<Longrightarrow> u = nth(succ(length(env)
 
 definition
   sep_var :: "i \<Rightarrow> i" where
-  "sep_var(n) \<equiv> {\<langle>0,1\<rangle>,\<langle>1,3\<rangle>,\<langle>2,4\<rangle>,\<langle>3,5\<rangle>,\<langle>4,0\<rangle>,\<langle>5#+n,6\<rangle>,\<langle>6#+n,2\<rangle>}"
+  "sep_var(n) \<equiv> {\<langle>0,1\<rangle>,\<langle>1,3\<rangle>,\<langle>2,4\<rangle>,\<langle>3,5\<rangle>,\<langle>4,0\<rangle>,\<langle>5+\<^sub>\<omega>n,6\<rangle>,\<langle>6+\<^sub>\<omega>n,2\<rangle>}"
 
 definition
   sep_env :: "i \<Rightarrow> i" where
-  "sep_env(n) \<equiv> \<lambda> i \<in> (5#+n)-5 . i#+2"
+  "sep_env(n) \<equiv> \<lambda> i \<in> (5+\<^sub>\<omega>n)-5 . i+\<^sub>\<omega>2"
 
 definition weak :: "[i, i] \<Rightarrow> i" where
-  "weak(n,m) \<equiv> {i#+m . i \<in> n}"
+  "weak(n,m) \<equiv> {i+\<^sub>\<omega>m . i \<in> n}"
 
 lemma weakD :
   assumes "n \<in> nat" "k\<in>nat" "x \<in> weak(n,k)"
-  shows "\<exists> i \<in> n . x = i#+k"
+  shows "\<exists> i \<in> n . x = i+\<^sub>\<omega>k"
   using assms unfolding weak_def by blast
 
 lemma weak_equal :
   assumes "n\<in>nat" "m\<in>nat"
-  shows "weak(n,m) = (m#+n) - m"
+  shows "weak(n,m) = (m+\<^sub>\<omega>n) - m"
 proof -
-  have "weak(n,m)\<subseteq>(m#+n)-m"
+  have "weak(n,m)\<subseteq>(m+\<^sub>\<omega>n)-m"
   proof(intro subsetI)
     fix x
     assume "x\<in>weak(n,m)"
     with assms
     obtain i where
-      "i\<in>n" "x=i#+m"
+      "i\<in>n" "x=i+\<^sub>\<omega>m"
       using weakD by blast
     then
-    have "m\<le>i#+m" "i<n"
+    have "m\<le>i+\<^sub>\<omega>m" "i<n"
       using add_le_self2[of m i] \<open>m\<in>nat\<close> \<open>n\<in>nat\<close> ltI[OF \<open>i\<in>n\<close>] by simp_all
     then
-    have "\<not>i#+m<m"
+    have "\<not>i+\<^sub>\<omega>m<m"
       using not_lt_iff_le in_n_in_nat[OF \<open>n\<in>nat\<close> \<open>i\<in>n\<close>] \<open>m\<in>nat\<close> by simp
-    with \<open>x=i#+m\<close>
+    with \<open>x=i+\<^sub>\<omega>m\<close>
     have "x\<notin>m"
       using ltI \<open>m\<in>nat\<close> by auto
     moreover
-    from assms \<open>x=i#+m\<close> \<open>i<n\<close>
-    have "x<m#+n"
+    from assms \<open>x=i+\<^sub>\<omega>m\<close> \<open>i<n\<close>
+    have "x<m+\<^sub>\<omega>n"
       using add_lt_mono1[OF \<open>i<n\<close> \<open>n\<in>nat\<close>] by simp
     ultimately
-    show "x\<in>(m#+n)-m"
+    show "x\<in>(m+\<^sub>\<omega>n)-m"
       using ltD DiffI by simp
   qed
   moreover
-  have "(m#+n)-m\<subseteq>weak(n,m)"
+  have "(m+\<^sub>\<omega>n)-m\<subseteq>weak(n,m)"
   proof (intro subsetI)
     fix x
-    assume "x\<in>(m#+n)-m"
+    assume "x\<in>(m+\<^sub>\<omega>n)-m"
     then
-    have "x\<in>m#+n" "x\<notin>m"
-      using DiffD1[of x "n#+m" m] DiffD2[of x "n#+m" m] by simp_all
+    have "x\<in>m+\<^sub>\<omega>n" "x\<notin>m"
+      using DiffD1[of x "n+\<^sub>\<omega>m" m] DiffD2[of x "n+\<^sub>\<omega>m" m] by simp_all
     then
-    have "x<m#+n" "x\<in>nat"
+    have "x<m+\<^sub>\<omega>n" "x\<in>nat"
       using ltI in_n_in_nat[OF add_type[of m n]] by simp_all
     then
     obtain i where
-      "m#+n = succ(x#+i)"
-      using less_iff_succ_add[OF \<open>x\<in>nat\<close>,of "m#+n"] add_type by auto
+      "m+\<^sub>\<omega>n = succ(x+\<^sub>\<omega>i)"
+      using less_iff_succ_add[OF \<open>x\<in>nat\<close>,of "m+\<^sub>\<omega>n"] add_type by auto
     then
-    have "x#+i<m#+n" using succ_le_iff by simp
+    have "x+\<^sub>\<omega>i<m+\<^sub>\<omega>n" using succ_le_iff by simp
     with \<open>x\<notin>m\<close>
     have "\<not>x<m" using ltD by blast
     with \<open>m\<in>nat\<close> \<open>x\<in>nat\<close>
     have "m\<le>x" using not_lt_iff_le by simp
-    with \<open>x<m#+n\<close>  \<open>n\<in>nat\<close>
-    have "x#-m<m#+n#-m"
+    with \<open>x<m+\<^sub>\<omega>n\<close>  \<open>n\<in>nat\<close>
+    have "x-\<^sub>\<omega>m<m+\<^sub>\<omega>n-\<^sub>\<omega>m"
       using diff_mono[OF \<open>x\<in>nat\<close> _ \<open>m\<in>nat\<close>] by simp
-    have "m#+n#-m =  n" using diff_cancel2 \<open>m\<in>nat\<close> \<open>n\<in>nat\<close> by simp
-    with \<open>x#-m<m#+n#-m\<close> \<open>x\<in>nat\<close>
-    have "x#-m \<in> n" "x=x#-m#+m"
+    have "m+\<^sub>\<omega>n-\<^sub>\<omega>m =  n" using diff_cancel2 \<open>m\<in>nat\<close> \<open>n\<in>nat\<close> by simp
+    with \<open>x-\<^sub>\<omega>m<m+\<^sub>\<omega>n-\<^sub>\<omega>m\<close> \<open>x\<in>nat\<close>
+    have "x-\<^sub>\<omega>m \<in> n" "x=x-\<^sub>\<omega>m+\<^sub>\<omega>m"
       using ltD add_diff_inverse2[OF \<open>m\<le>x\<close>] by simp_all
     then
     show "x\<in>weak(n,m)"
@@ -102,7 +102,7 @@ lemma weak_zero:
 
 lemma weakening_diff :
   assumes "n \<in> nat"
-  shows "weak(n,7) - weak(n,5) \<subseteq> {5#+n, 6#+n}"
+  shows "weak(n,7) - weak(n,5) \<subseteq> {5+\<^sub>\<omega>n, 6+\<^sub>\<omega>n}"
   unfolding weak_def using assms
 proof(auto)
   {
@@ -157,31 +157,31 @@ proof(auto)
 qed
 
 lemma in_add_del :
-  assumes "x\<in>j#+n" "n\<in>nat" "j\<in>nat"
+  assumes "x\<in>j+\<^sub>\<omega>n" "n\<in>nat" "j\<in>nat"
   shows "x < j \<or> x \<in> weak(n,j)"
 proof (cases "x<j")
   case True
   then show ?thesis ..
 next
   case False
-  have "x\<in>nat" "j#+n\<in>nat"
-    using in_n_in_nat[OF _ \<open>x\<in>j#+n\<close>] assms by simp_all
+  have "x\<in>nat" "j+\<^sub>\<omega>n\<in>nat"
+    using in_n_in_nat[OF _ \<open>x\<in>j+\<^sub>\<omega>n\<close>] assms by simp_all
   then
-  have "j \<le> x" "x < j#+n"
-    using not_lt_iff_le False \<open>j\<in>nat\<close> \<open>n\<in>nat\<close> ltI[OF \<open>x\<in>j#+n\<close>] by auto
+  have "j \<le> x" "x < j+\<^sub>\<omega>n"
+    using not_lt_iff_le False \<open>j\<in>nat\<close> \<open>n\<in>nat\<close> ltI[OF \<open>x\<in>j+\<^sub>\<omega>n\<close>] by auto
   then
-  have "x#-j < (j #+ n) #- j" "x = j #+ (x #-j)"
-    using diff_mono \<open>x\<in>nat\<close> \<open>j#+n\<in>nat\<close> \<open>j\<in>nat\<close> \<open>n\<in>nat\<close>
+  have "x-\<^sub>\<omega>j < (j +\<^sub>\<omega> n) -\<^sub>\<omega> j" "x = j +\<^sub>\<omega> (x -\<^sub>\<omega>j)"
+    using diff_mono \<open>x\<in>nat\<close> \<open>j+\<^sub>\<omega>n\<in>nat\<close> \<open>j\<in>nat\<close> \<open>n\<in>nat\<close>
       add_diff_inverse[OF \<open>j\<le>x\<close>] by simp_all
   then
-  have "x#-j < n" "x = (x #-j ) #+ j"
+  have "x-\<^sub>\<omega>j < n" "x = (x -\<^sub>\<omega>j ) +\<^sub>\<omega> j"
     using diff_add_inverse \<open>n\<in>nat\<close> add_commute by simp_all
   then
-  have "x#-j \<in>n" using ltD by simp
+  have "x-\<^sub>\<omega>j \<in>n" using ltD by simp
   then
   have "x \<in> weak(n,j)"
     unfolding weak_def
-    using \<open>x= (x#-j) #+j\<close> RepFunI[OF \<open>x#-j\<in>n\<close>] add_commute by force
+    using \<open>x= (x-\<^sub>\<omega>j) +\<^sub>\<omega>j\<close> RepFunI[OF \<open>x-\<^sub>\<omega>j\<in>n\<close>] add_commute by force
   then show ?thesis  ..
 qed
 
@@ -194,47 +194,47 @@ lemma sep_env_action:
       nth(sep_env(length(env))`i,[t,p,u,P,leq,o,pi]@env) = nth(i,[p,P,leq,o,t] @ env @ [pi,u])"
 proof -
   from assms
-  have A: "5#+length(env)\<in>nat" "[p, P, leq, o, t] \<in>list(M)"
+  have A: "5+\<^sub>\<omega>length(env)\<in>nat" "[p, P, leq, o, t] \<in>list(M)"
     by simp_all
   let ?f="sep_env(length(env))"
-  have EQ: "weak(length(env),5) = 5#+length(env) - 5"
+  have EQ: "weak(length(env),5) = 5+\<^sub>\<omega>length(env) - 5"
     using weak_equal length_type[OF \<open>env\<in>list(M)\<close>] by simp
   let ?tgt="[t,p,u,P,leq,o,pi]@env"
   let ?src="[p,P,leq,o,t] @ env @ [pi,u]"
   have "nth(?f`i,[t,p,u,P,leq,o,pi]@env) = nth(i,[p,P,leq,o,t] @ env @ [pi,u])"
-    if "i \<in> (5#+length(env)-5)" for i
+    if "i \<in> (5+\<^sub>\<omega>length(env)-5)" for i
   proof -
     from that
-    have 2: "i \<in> 5#+length(env)"  "i \<notin> 5" "i \<in> nat" "i#-5\<in>nat" "i#+2\<in>nat"
-      using in_n_in_nat[OF \<open>5#+length(env)\<in>nat\<close>] by simp_all
+    have 2: "i \<in> 5+\<^sub>\<omega>length(env)"  "i \<notin> 5" "i \<in> nat" "i-\<^sub>\<omega>5\<in>nat" "i+\<^sub>\<omega>2\<in>nat"
+      using in_n_in_nat[OF \<open>5+\<^sub>\<omega>length(env)\<in>nat\<close>] by simp_all
     then
     have 3: "\<not> i < 5" using ltD by force
     then
     have "5 \<le> i" "2 \<le> 5"
       using  not_lt_iff_le \<open>i\<in>nat\<close> by simp_all
     then have "2 \<le> i" using le_trans[OF \<open>2\<le>5\<close>] by simp
-    from A \<open>i \<in> 5#+length(env)\<close>
-    have "i < 5#+length(env)" using ltI by simp
+    from A \<open>i \<in> 5+\<^sub>\<omega>length(env)\<close>
+    have "i < 5+\<^sub>\<omega>length(env)" using ltI by simp
     with \<open>i\<in>nat\<close> \<open>2\<le>i\<close> A
-    have C:"i#+2 < 7#+length(env)"  by simp
+    have C:"i+\<^sub>\<omega>2 < 7+\<^sub>\<omega>length(env)"  by simp
     with that
-    have B: "?f`i = i#+2" unfolding sep_env_def by simp
+    have B: "?f`i = i+\<^sub>\<omega>2" unfolding sep_env_def by simp
     from 3 assms(1) \<open>i\<in>nat\<close>
-    have "\<not> i#+2 < 7" using not_lt_iff_le add_le_mono by simp
-    from \<open>i < 5#+length(env)\<close> 3 \<open>i\<in>nat\<close>
-    have "i#-5 < 5#+length(env) #- 5"
-      using diff_mono[of i "5#+length(env)" 5,OF _ _ _ \<open>i < 5#+length(env)\<close>]
+    have "\<not> i+\<^sub>\<omega>2 < 7" using not_lt_iff_le add_le_mono by simp
+    from \<open>i < 5+\<^sub>\<omega>length(env)\<close> 3 \<open>i\<in>nat\<close>
+    have "i-\<^sub>\<omega>5 < 5+\<^sub>\<omega>length(env) -\<^sub>\<omega> 5"
+      using diff_mono[of i "5+\<^sub>\<omega>length(env)" 5,OF _ _ _ \<open>i < 5+\<^sub>\<omega>length(env)\<close>]
         not_lt_iff_le[THEN iffD1] by force
     with assms(2)
-    have "i#-5 < length(env)" using diff_add_inverse length_type by simp
-    have "nth(i,?src) =nth(i#-5,env@[pi,u])"
+    have "i-\<^sub>\<omega>5 < length(env)" using diff_add_inverse length_type by simp
+    have "nth(i,?src) =nth(i-\<^sub>\<omega>5,env@[pi,u])"
       using nth_append[OF A(2) \<open>i\<in>nat\<close>] 3 by simp
     also
-    have "... = nth(i#-5, env)"
-      using nth_append[OF \<open>env \<in>list(M)\<close> \<open>i#-5\<in>nat\<close>] \<open>i#-5 < length(env)\<close> by simp
+    have "... = nth(i-\<^sub>\<omega>5, env)"
+      using nth_append[OF \<open>env \<in>list(M)\<close> \<open>i-\<^sub>\<omega>5\<in>nat\<close>] \<open>i-\<^sub>\<omega>5 < length(env)\<close> by simp
     also
-    have "... = nth(i#+2, ?tgt)"
-      using nth_append[OF assms(1) \<open>i#+2\<in>nat\<close>] \<open>\<not> i#+2 <7\<close> by simp
+    have "... = nth(i+\<^sub>\<omega>2, ?tgt)"
+      using nth_append[OF assms(1) \<open>i+\<^sub>\<omega>2\<in>nat\<close>] \<open>\<not> i+\<^sub>\<omega>2 <7\<close> by simp
     ultimately
     have "nth(i,?src) = nth(?f`i,?tgt)"
       using B by simp
@@ -245,93 +245,93 @@ qed
 
 lemma sep_env_type :
   assumes "n \<in> nat"
-  shows "sep_env(n) : (5#+n)-5 \<rightarrow> (7#+n)-7"
+  shows "sep_env(n) : (5+\<^sub>\<omega>n)-5 \<rightarrow> (7+\<^sub>\<omega>n)-7"
 proof -
   let ?h="sep_env(n)"
   from \<open>n\<in>nat\<close>
-  have "(5#+n)#+2 = 7#+n" "7#+n\<in>nat" "5#+n\<in>nat" by simp_all
+  have "(5+\<^sub>\<omega>n)+\<^sub>\<omega>2 = 7+\<^sub>\<omega>n" "7+\<^sub>\<omega>n\<in>nat" "5+\<^sub>\<omega>n\<in>nat" by simp_all
   have
-    D: "sep_env(n)`x \<in> (7#+n)-7" if "x \<in> (5#+n)-5" for x
+    D: "sep_env(n)`x \<in> (7+\<^sub>\<omega>n)-7" if "x \<in> (5+\<^sub>\<omega>n)-5" for x
   proof -
-    from \<open>x\<in>5#+n-5\<close>
-    have "?h`x = x#+2" "x<5#+n" "x\<in>nat"
-      unfolding sep_env_def using ltI in_n_in_nat[OF \<open>5#+n\<in>nat\<close>] by simp_all
+    from \<open>x\<in>5+\<^sub>\<omega>n-5\<close>
+    have "?h`x = x+\<^sub>\<omega>2" "x<5+\<^sub>\<omega>n" "x\<in>nat"
+      unfolding sep_env_def using ltI in_n_in_nat[OF \<open>5+\<^sub>\<omega>n\<in>nat\<close>] by simp_all
     then
-    have "x#+2 < 7#+n" by simp
+    have "x+\<^sub>\<omega>2 < 7+\<^sub>\<omega>n" by simp
     then
-    have "x#+2 \<in> 7#+n" using ltD by simp
-    from \<open>x\<in>5#+n-5\<close>
+    have "x+\<^sub>\<omega>2 \<in> 7+\<^sub>\<omega>n" using ltD by simp
+    from \<open>x\<in>5+\<^sub>\<omega>n-5\<close>
     have "x\<notin>5" by simp
     then have "\<not>x<5" using ltD by blast
     then have "5\<le>x" using not_lt_iff_le \<open>x\<in>nat\<close> by simp
-    then have "7\<le>x#+2" using add_le_mono \<open>x\<in>nat\<close> by simp
-    then have "\<not>x#+2<7" using not_lt_iff_le \<open>x\<in>nat\<close> by simp
-    then have "x#+2 \<notin> 7" using ltI \<open>x\<in>nat\<close> by force
-    with \<open>x#+2 \<in> 7#+n\<close> show ?thesis using  \<open>?h`x = x#+2\<close> DiffI by simp
+    then have "7\<le>x+\<^sub>\<omega>2" using add_le_mono \<open>x\<in>nat\<close> by simp
+    then have "\<not>x+\<^sub>\<omega>2<7" using not_lt_iff_le \<open>x\<in>nat\<close> by simp
+    then have "x+\<^sub>\<omega>2 \<notin> 7" using ltI \<open>x\<in>nat\<close> by force
+    with \<open>x+\<^sub>\<omega>2 \<in> 7+\<^sub>\<omega>n\<close> show ?thesis using  \<open>?h`x = x+\<^sub>\<omega>2\<close> DiffI by simp
   qed
   then show ?thesis unfolding sep_env_def using lam_type by simp
 qed
 
 lemma sep_var_fin_type :
   assumes "n \<in> nat"
-  shows "sep_var(n) : 7#+n  -||> 7#+n"
+  shows "sep_var(n) : 7+\<^sub>\<omega>n  -||> 7+\<^sub>\<omega>n"
   unfolding sep_var_def
   using consI ltD emptyI by force
 
 lemma sep_var_domain :
   assumes "n \<in> nat"
-  shows "domain(sep_var(n)) =  7#+n - weak(n,5)"
+  shows "domain(sep_var(n)) =  7+\<^sub>\<omega>n - weak(n,5)"
 proof -
   let ?A="weak(n,5)"
-  have A:"domain(sep_var(n)) \<subseteq> (7#+n)"
+  have A:"domain(sep_var(n)) \<subseteq> (7+\<^sub>\<omega>n)"
     unfolding sep_var_def
     by(auto simp add: le_natE)
-  have C: "x=5#+n \<or> x=6#+n \<or> x \<le> 4" if "x\<in>domain(sep_var(n))" for x
+  have C: "x=5+\<^sub>\<omega>n \<or> x=6+\<^sub>\<omega>n \<or> x \<le> 4" if "x\<in>domain(sep_var(n))" for x
     using that unfolding sep_var_def by auto
-  have D : "x<n#+7" if "x\<in>7#+n" for x
+  have D : "x<n+\<^sub>\<omega>7" if "x\<in>7+\<^sub>\<omega>n" for x
     using that \<open>n\<in>nat\<close> ltI by simp
-  have "\<not> 5#+n < 5#+n" using \<open>n\<in>nat\<close>  lt_irrefl[of _ False] by force
-  have "\<not> 6#+n < 5#+n" using \<open>n\<in>nat\<close> by force
-  have R: "x < 5#+n" if "x\<in>?A" for x
+  have "\<not> 5+\<^sub>\<omega>n < 5+\<^sub>\<omega>n" using \<open>n\<in>nat\<close>  lt_irrefl[of _ False] by force
+  have "\<not> 6+\<^sub>\<omega>n < 5+\<^sub>\<omega>n" using \<open>n\<in>nat\<close> by force
+  have R: "x < 5+\<^sub>\<omega>n" if "x\<in>?A" for x
   proof -
     from that
     obtain i where
-      "i<n" "x=5#+i"
+      "i<n" "x=5+\<^sub>\<omega>i"
       unfolding weak_def
       using ltI \<open>n\<in>nat\<close> RepFun_iff by force
     with \<open>n\<in>nat\<close>
-    have "5#+i < 5#+n" using add_lt_mono2 by simp
-    with \<open>x=5#+i\<close>
-    show "x < 5#+n" by simp
+    have "5+\<^sub>\<omega>i < 5+\<^sub>\<omega>n" using add_lt_mono2 by simp
+    with \<open>x=5+\<^sub>\<omega>i\<close>
+    show "x < 5+\<^sub>\<omega>n" by simp
   qed
   then
-  have 1:"x\<notin>?A" if "\<not>x <5#+n" for x using that by blast
-  have "5#+n \<notin> ?A" "6#+n\<notin>?A"
+  have 1:"x\<notin>?A" if "\<not>x <5+\<^sub>\<omega>n" for x using that by blast
+  have "5+\<^sub>\<omega>n \<notin> ?A" "6+\<^sub>\<omega>n\<notin>?A"
   proof -
-    show "5#+n \<notin> ?A" using 1 \<open>\<not>5#+n<5#+n\<close> by blast
-    with 1 show "6#+n \<notin> ?A" using  \<open>\<not>6#+n<5#+n\<close> by blast
+    show "5+\<^sub>\<omega>n \<notin> ?A" using 1 \<open>\<not>5+\<^sub>\<omega>n<5+\<^sub>\<omega>n\<close> by blast
+    with 1 show "6+\<^sub>\<omega>n \<notin> ?A" using  \<open>\<not>6+\<^sub>\<omega>n<5+\<^sub>\<omega>n\<close> by blast
   qed
   then
   have E:"x\<notin>?A" if "x\<in>domain(sep_var(n))" for x
     unfolding weak_def
     using C that by force
   then
-  have F: "domain(sep_var(n)) \<subseteq> 7#+n - ?A" using A by auto
+  have F: "domain(sep_var(n)) \<subseteq> 7+\<^sub>\<omega>n - ?A" using A by auto
   from assms
-  have "x<7 \<or> x\<in>weak(n,7)" if "x\<in>7#+n" for x
-    using in_add_del[OF \<open>x\<in>7#+n\<close>] by simp
+  have "x<7 \<or> x\<in>weak(n,7)" if "x\<in>7+\<^sub>\<omega>n" for x
+    using in_add_del[OF \<open>x\<in>7+\<^sub>\<omega>n\<close>] by simp
   moreover
   {
     fix x
-    assume asm:"x\<in>7#+n"  "x\<notin>?A"  "x\<in>weak(n,7)"
+    assume asm:"x\<in>7+\<^sub>\<omega>n"  "x\<notin>?A"  "x\<in>weak(n,7)"
     then
     have "x\<in>domain(sep_var(n))"
     proof -
       from \<open>n\<in>nat\<close>
-      have "weak(n,7)-weak(n,5)\<subseteq>{n#+5,n#+6}"
+      have "weak(n,7)-weak(n,5)\<subseteq>{n+\<^sub>\<omega>5,n+\<^sub>\<omega>6}"
         using weakening_diff by simp
       with  \<open>x\<notin>?A\<close> asm
-      have "x\<in>{n#+5,n#+6}" using  subsetD DiffI by blast
+      have "x\<in>{n+\<^sub>\<omega>5,n+\<^sub>\<omega>6}" using  subsetD DiffI by blast
       then
       show ?thesis unfolding sep_var_def by simp
     qed
@@ -339,7 +339,7 @@ proof -
   moreover
   {
     fix x
-    assume asm:"x\<in>7#+n"  "x\<notin>?A" "x<7"
+    assume asm:"x\<in>7+\<^sub>\<omega>n"  "x\<notin>?A" "x<7"
     then have "x\<in>domain(sep_var(n))"
     proof (cases "2 \<le> n")
       case True
@@ -377,17 +377,17 @@ proof -
     qed
   }
   ultimately
-  have "w\<in>domain(sep_var(n))" if "w\<in> 7#+n - ?A" for w
+  have "w\<in>domain(sep_var(n))" if "w\<in> 7+\<^sub>\<omega>n - ?A" for w
     using that by blast
   then
-  have "7#+n - ?A \<subseteq> domain(sep_var(n))" by blast
+  have "7+\<^sub>\<omega>n - ?A \<subseteq> domain(sep_var(n))" by blast
   with F
   show ?thesis by auto
 qed
 
 lemma sep_var_type :
   assumes "n \<in> nat"
-  shows "sep_var(n) : (7#+n)-weak(n,5) \<rightarrow> 7#+n"
+  shows "sep_var(n) : (7+\<^sub>\<omega>n)-weak(n,5) \<rightarrow> 7+\<^sub>\<omega>n"
   using FiniteFun_is_fun[OF sep_var_fin_type[OF \<open>n\<in>nat\<close>]]
     sep_var_domain[OF \<open>n\<in>nat\<close>] by simp
 
@@ -395,7 +395,7 @@ lemma sep_var_action :
   assumes
     "[t,p,u,P,leq,o,pi] \<in> list(M)"
     "env \<in> list(M)"
-  shows "\<forall> i . i \<in> (7#+length(env)) - weak(length(env),5) \<longrightarrow>
+  shows "\<forall> i . i \<in> (7+\<^sub>\<omega>length(env)) - weak(length(env),5) \<longrightarrow>
     nth(sep_var(length(env))`i,[t,p,u,P,leq,o,pi]@env) = nth(i,[p,P,leq,o,t] @ env @ [pi,u])"
   using assms
 proof (subst sep_var_domain[OF length_type[OF \<open>env\<in>list(M)\<close>],symmetric],auto)
@@ -413,26 +413,26 @@ proof (subst sep_var_domain[OF length_type[OF \<open>env\<in>list(M)\<close>],sy
 
 definition
   rensep :: "i \<Rightarrow> i" where
-  "rensep(n) \<equiv> union_fun(sep_var(n),sep_env(n),7#+n-weak(n,5),weak(n,5))"
+  "rensep(n) \<equiv> union_fun(sep_var(n),sep_env(n),7+\<^sub>\<omega>n-weak(n,5),weak(n,5))"
 
 lemma rensep_aux :
   assumes "n\<in>nat"
-  shows "(7#+n-weak(n,5)) \<union> weak(n,5) = 7#+n" "7#+n \<union> ( 7 #+ n - 7) = 7#+n"
+  shows "(7+\<^sub>\<omega>n-weak(n,5)) \<union> weak(n,5) = 7+\<^sub>\<omega>n" "7+\<^sub>\<omega>n \<union> ( 7 +\<^sub>\<omega> n - 7) = 7+\<^sub>\<omega>n"
 proof -
   from \<open>n\<in>nat\<close>
-  have "weak(n,5) = n#+5-5"
+  have "weak(n,5) = n+\<^sub>\<omega>5-5"
     using weak_equal by simp
   with  \<open>n\<in>nat\<close>
-  show "(7#+n-weak(n,5)) \<union> weak(n,5) = 7#+n" "7#+n \<union> ( 7 #+ n - 7) = 7#+n"
+  show "(7+\<^sub>\<omega>n-weak(n,5)) \<union> weak(n,5) = 7+\<^sub>\<omega>n" "7+\<^sub>\<omega>n \<union> ( 7 +\<^sub>\<omega> n - 7) = 7+\<^sub>\<omega>n"
     using Diff_partition le_imp_subset by auto
 qed
 
 lemma rensep_type :
   assumes "n\<in>nat"
-  shows "rensep(n) \<in> 7#+n \<rightarrow> 7#+n"
+  shows "rensep(n) \<in> 7+\<^sub>\<omega>n \<rightarrow> 7+\<^sub>\<omega>n"
 proof -
   from \<open>n\<in>nat\<close>
-  have "rensep(n) \<in> (7#+n-weak(n,5)) \<union> weak(n,5) \<rightarrow> 7#+n \<union> (7#+n - 7)"
+  have "rensep(n) \<in> (7+\<^sub>\<omega>n-weak(n,5)) \<union> weak(n,5) \<rightarrow> 7+\<^sub>\<omega>n \<union> (7+\<^sub>\<omega>n - 7)"
     unfolding rensep_def
     using union_fun_type  sep_var_type \<open>n\<in>nat\<close> sep_env_type weak_equal
     by force
@@ -442,11 +442,11 @@ qed
 
 lemma rensep_action :
   assumes "[t,p,u,P,leq,o,pi] @ env \<in> list(M)"
-  shows "\<forall> i . i < 7#+length(env) \<longrightarrow> nth(rensep(length(env))`i,[t,p,u,P,leq,o,pi]@env) = nth(i,[p,P,leq,o,t] @ env @ [pi,u])"
+  shows "\<forall> i . i < 7+\<^sub>\<omega>length(env) \<longrightarrow> nth(rensep(length(env))`i,[t,p,u,P,leq,o,pi]@env) = nth(i,[p,P,leq,o,t] @ env @ [pi,u])"
 proof -
   let ?tgt="[t,p,u,P,leq,o,pi]@env"
   let ?src="[p,P,leq,o,t] @ env @ [pi,u]"
-  let ?m="7 #+ length(env) - weak(length(env),5)"
+  let ?m="7 +\<^sub>\<omega> length(env) - weak(length(env),5)"
   let ?p="weak(length(env),5)"
   let ?f="sep_var(length(env))"
   let ?g="sep_env(length(env))"
@@ -454,18 +454,18 @@ proof -
   from assms
   have 1 : "[t,p,u,P,leq,o,pi] \<in> list(M)" " env \<in> list(M)"
     "?src \<in> list(M)" "?tgt \<in> list(M)"
-    "7#+?n = (7#+?n-weak(?n,5)) \<union> weak(?n,5)"
-    " length(?src) = (7#+?n-weak(?n,5)) \<union> weak(?n,5)"
+    "7+\<^sub>\<omega>?n = (7+\<^sub>\<omega>?n-weak(?n,5)) \<union> weak(?n,5)"
+    " length(?src) = (7+\<^sub>\<omega>?n-weak(?n,5)) \<union> weak(?n,5)"
     using Diff_partition le_imp_subset rensep_aux by auto
   then
-  have "nth(i, ?src) = nth(union_fun(?f, ?g, ?m, ?p) ` i, ?tgt)" if "i < 7#+length(env)" for i
+  have "nth(i, ?src) = nth(union_fun(?f, ?g, ?m, ?p) ` i, ?tgt)" if "i < 7+\<^sub>\<omega>length(env)" for i
   proof -
-    from \<open>i<7#+?n\<close>
-    have "i \<in> (7#+?n-weak(?n,5)) \<union> weak(?n,5)"
+    from \<open>i<7+\<^sub>\<omega>?n\<close>
+    have "i \<in> (7+\<^sub>\<omega>?n-weak(?n,5)) \<union> weak(?n,5)"
       using ltD by simp
     then show ?thesis
       unfolding rensep_def using
-        union_fun_action[OF \<open>?src\<in>list(M)\<close> \<open>?tgt\<in>list(M)\<close> \<open>length(?src) = (7#+?n-weak(?n,5)) \<union> weak(?n,5)\<close>
+        union_fun_action[OF \<open>?src\<in>list(M)\<close> \<open>?tgt\<in>list(M)\<close> \<open>length(?src) = (7+\<^sub>\<omega>?n-weak(?n,5)) \<union> weak(?n,5)\<close>
           sep_var_action[OF \<open>[t,p,u,P,leq,o,pi] \<in> list(M)\<close> \<open>env\<in>list(M)\<close>]
           sep_env_action[OF \<open>[t,p,u,P,leq,o,pi] \<in> list(M)\<close> \<open>env\<in>list(M)\<close>]
           ] that
@@ -475,11 +475,11 @@ proof -
 qed
 
 definition sep_ren :: "[i,i] \<Rightarrow> i" where
-  "sep_ren(n,\<phi>) \<equiv> ren(\<phi>)`(7#+n)`(7#+n)`rensep(n)"
+  "sep_ren(n,\<phi>) \<equiv> ren(\<phi>)`(7+\<^sub>\<omega>n)`(7+\<^sub>\<omega>n)`rensep(n)"
 
 lemma arity_rensep: assumes "\<phi>\<in>formula" "env \<in> list(M)"
-  "arity(\<phi>) \<le> 7#+length(env)"
-shows "arity(sep_ren(length(env),\<phi>)) \<le> 7#+length(env)"
+  "arity(\<phi>) \<le> 7+\<^sub>\<omega>length(env)"
+shows "arity(sep_ren(length(env),\<phi>)) \<le> 7+\<^sub>\<omega>length(env)"
   unfolding sep_ren_def
   using arity_ren rensep_type assms
   by simp
@@ -492,7 +492,7 @@ lemma type_rensep [TC]:
   by simp
 
 lemma sepren_action:
-  assumes "arity(\<phi>) \<le> 7 #+ length(env)"
+  assumes "arity(\<phi>) \<le> 7 +\<^sub>\<omega> length(env)"
     "[t,p,u,P,leq,o,pi] \<in> list(M)"
     "env\<in>list(M)"
     "\<phi>\<in>formula"
@@ -512,7 +512,7 @@ proof -
         add_type[of 7 "length(env)"]
         2 1(1)
         rensep_type[OF length_type[OF \<open>env\<in>list(M)\<close>]]
-        \<open>arity(\<phi>) \<le> 7 #+ length(env)\<close>]
+        \<open>arity(\<phi>) \<le> 7 +\<^sub>\<omega> length(env)\<close>]
       rensep_action[OF 1(1),rule_format,symmetric]
     by simp
 qed
